make PROP in Handler explicit and Event -> Effect

IrisITree/IrisITree/Core/Handler.lean
@@ -10,10 +10,10 @@ open Iris BI ITree
 
 /-
   An [IHandler] is the user-specified recipe used to define a custom
-  weakest precondition [WPi]. It specifies how to interpret an event
+  weakest precondition [WPi]. It specifies how to interpret an effect
   logically, given weakest preconditions for continuations of the itree.
 -/
-structure IHandler {PROP} [BI PROP] (E : Effect.{u}) where
+structure IHandler (PROP) [BI PROP] (E : Effect.{u}) where
   ihandle :
       (i : E.I) →
       -- Continuation conditions [λ a, ▷ WPi k a @ H; ∅ {{ Φ }}]
@@ -29,7 +29,7 @@ structure IHandler {PROP} [BI PROP] (E : Effect.{u}) where
       □ (∀ t, s t -∗ s' t) -∗
       ihandle i Φ s -∗ ihandle i Φ' s'
 
-instance {PROP E} [BI PROP] (H : IHandler (PROP := PROP) E) (i : E.I) :
+instance {PROP E} [BI PROP] (H : IHandler PROP E) (i : E.I) :
     OFE.NonExpansive₂ (H.ihandle i) := by
   constructor
   intro n Φ₁ Φ₂ HΦ s₁ s₂ Hs
@@ -49,10 +49,10 @@ instance {PROP E} [BI PROP] (H : IHandler (PROP := PROP) E) (i : E.I) :
 
 section handler_sumH
 
-variable {E₁ E₂} {PROP : Type _} [BI PROP] (H₁ : IHandler (PROP := PROP) E₁) (H₂ : IHandler (PROP := PROP) E₂)
+variable {E₁ E₂} {PROP : Type _} [BI PROP] (H₁ : IHandler PROP E₁) (H₂ : IHandler PROP E₂)
 
 -- An [IHandler] for sum events [E₁ ⊕ₑ E₂] delegating to respective [IHandler]s.
-def sumH : IHandler (PROP := PROP) (E₁ ⊕ₑ E₂) where
+def sumH : IHandler PROP (E₁ ⊕ₑ E₂) where
   ihandle := by
     intro e Φ s
     cases e with
@@ -77,18 +77,18 @@ variable {PROP : Type _} [BI PROP]
 
 /- `InH H1 H2` means that, on events [E1], [H1] is equivalent to [H2] -/
 class InH {E₁ E₂} [Hsub : E₁ -< E₂]
-    (H1 : IHandler (PROP := PROP) E₁) (H2 : IHandler (PROP := PROP) E₂) where
+    (H1 : IHandler PROP E₁) (H2 : IHandler PROP E₂) where
   is_inH : ∀ (i₁ : E₁.I) (Φ₁ s₁ : E₁.O i₁ → PROP),
     let ⟨i₂, f⟩ := Hsub.map i₁
     let Φ₂ := fun x => Φ₁ <| f x
     let s₂ := fun x => s₁ <| f x
     H1.ihandle i₁ Φ₁ s₁ ⊣⊢ H2.ihandle i₂ Φ₂ s₂
 
-instance {PROP E} [BI PROP] (H : IHandler (PROP := PROP) E) : InH H H := by
+instance {PROP E} [BI PROP] (H : IHandler PROP E) : InH H H := by
   constructor; intro i Φ s; simp
 
 instance {PROP E₁ E₂ E₃} [BI PROP] [f : E₁ -< E₂]
-    (H1 : IHandler (PROP := PROP) E₁) (H2 : IHandler (PROP := PROP) E₂) (H3 : IHandler (PROP := PROP) E₃) :
+    (H1 : IHandler PROP E₁) (H2 : IHandler PROP E₂) (H3 : IHandler PROP E₃) :
   InH H1 H2 → InH H1 (H2 ⊕ₕ H3) := by
     intro Hin
     constructor
@@ -96,7 +96,7 @@ instance {PROP E₁ E₂ E₃} [BI PROP] [f : E₁ -< E₂]
     exact Hin.is_inH i Φ s
 
 instance {PROP E₁ E₂ E₃} [BI PROP] [f : E₁ -< E₃]
-    (H1 : IHandler (PROP := PROP) E₁) (H2 : IHandler (PROP := PROP) E₂) (H3 : IHandler (PROP := PROP) E₃) :
+    (H1 : IHandler PROP E₁) (H2 : IHandler PROP E₂) (H3 : IHandler PROP E₃) :
   InH H1 H3 → InH H1 (H2 ⊕ₕ H3) := by
     intro Hin
     constructor
@@ -108,17 +108,17 @@ end handler_InH
 section handler_WandH
 
 /- `[WandH H1 H2]` means that `H1` implies `H2` -/
-class WandH {PROP E} [BI PROP] (H1 : IHandler (PROP := PROP) E) (H2 : IHandler (PROP := PROP) E) where
+class WandH {PROP E} [BI PROP] (H1 : IHandler PROP E) (H2 : IHandler PROP E) where
   is_wandH : ∀ (i : E.I) (Φ s : E.O i → PROP),
     ⊢ H1.ihandle i Φ s -∗ H2.ihandle i Φ s
 
-instance {PROP E} [BI PROP] (H : IHandler (PROP := PROP) E) : WandH H H := by
+instance {PROP E} [BI PROP] (H : IHandler PROP E) : WandH H H := by
   constructor
   iintro %i %Φ %s H
   iexact H
 
 instance {PROP E₁ E₂} [BI PROP]
-    (H1 H1' : IHandler (PROP := PROP) E₁) (H2 H2' : IHandler (PROP := PROP) E₂) :
+    (H1 H1' : IHandler PROP E₁) (H2 H2' : IHandler PROP E₂) :
   WandH H1 H1' → WandH H2 H2' → WandH (H1 ⊕ₕ H2) (H1' ⊕ₕ H2') := by
     intro Hwand1 Hwand2
     constructor
@@ -132,12 +132,12 @@ end handler_WandH
 section handler_Sequential
 
 /- `Sequential` handlers ignore the spawning continuation and do not model concurrency. -/
-class Sequential {PROP} [BI PROP] {E : Effect} (H : IHandler (PROP := PROP) E) where
+class Sequential {PROP} [BI PROP] {E : Effect} (H : IHandler PROP E) where
   is_seq : ∀ (i : E.I) (Φ s : E.O i → PROP),
     ⊢ H.ihandle i Φ s -∗ H.ihandle i Φ (fun _ => iprop(⌜False⌝))
 
 instance {PROP E₁ E₂} [BI PROP]
-  (H1 : IHandler (PROP := PROP) E₁) (H2 : IHandler (PROP := PROP) E₂)
+  (H1 : IHandler PROP E₁) (H2 : IHandler PROP E₂)
   [Hs1 : Sequential H1] [Hs2 : Sequential H2] : Sequential (H1 ⊕ₕ H2) := by
     refine ⟨?_⟩
     iintro %e %Φ %s H
