IrisITree/IrisITree.lean
@@ -1,6 +1,4 @@
 module
 
-public import ITree
-public import Iris
 public import IrisITree.Core
-public import IrisITree.Event
+public import IrisITree.Effect
