IrisITree/IrisITree/Effect/Empty.lean
@@ -5,7 +5,7 @@ public import ITree
 
 @[expose] public section
 
-namespace IrisITree.Event
+namespace IrisITree.Effect
 
 open Iris BI ITree Effects
 
@@ -14,7 +14,7 @@ section handler
 variable {PROP : Type _} [BI PROP]
 
 /-- The canonical handler for the empty event type. -/
-def emptyH : IHandler (PROP := PROP) emptyE where
+def emptyH : IHandler PROP emptyE where
   ihandle := by intro i; cases i
   ihandle_mono := by iintro %i; cases i
 
@@ -26,4 +26,4 @@ end handler
 def insert_emptyE {E R} (t : ITree E R) : ITree (E ⊕ₑ emptyE) R :=
   ITree.interp (fun i => ITree.trigger E i) t
 
-end IrisITree.Event
+end IrisITree.Effect
