IrisITree/IrisITree/ThreadPool/Handler.lean
@@ -1,5 +1,5 @@
 namespace IrisITree.ThreadPool
 
-/- Event handlers specialized to thread-pool concurrency. -/
+/- Effect handlers specialized to thread-pool concurrency. -/
 
 end IrisITree.ThreadPool
